\documentclass[../notes.tex]{subfiles}

\begin{document}
	\chapter{Proofs Involving Sets}
		\section{Venn Diagrams}
			\subsection{Set Equality}
				For any sets $A$ and $B$, if $A \subseteq B$ and $B \subseteq A$, then every element of $A$ is also an element of $B$, and every element of $B$ is also an element of $A$, so $A = B$.
			\subsection{Drawing Complex Venn Diagrams}
			Draw the diagram in stages, including $U$, $A$, $B$ and $C$ in each diagram.
			\begin{examplebox}
				Let $A$, $B$, $C \subseteq U$. Draw the Venn diagram for $\Bigl[(A \cup B) - (A \cap B)\Bigr] \cup C$
				\begin{enumerate}
					\item $A \cup B$
						\begin{center}
							\begin{venndiagram3sets}[shade=circle area, tikzoptions={myvennoutline}, showframe=false]
								\fillA
								\fillB
							\end{venndiagram3sets}
						\end{center}
						\pagebreak
					\item $A \cap B$
						\begin{center}
							\begin{venndiagram3sets}[shade=circle area, tikzoptions={myvennoutline}, showframe=false]
								\fillACapB
							\end{venndiagram3sets}
						\end{center}
					\item $(A \cup B) - (A \cap B)$
						\begin{center}
							\begin{venndiagram3sets}[shade=circle area, tikzoptions={myvennoutline}, showframe=false]
								\fillANotB
								\fillBNotA
							\end{venndiagram3sets}
						\end{center}
					\item $C$
						\begin{center}
							\begin{venndiagram3sets}[shade=circle area, tikzoptions={myvennoutline}, showframe=false]
								\fillC
							\end{venndiagram3sets}
						\end{center}
						\pagebreak
					\item $\Bigl[(A \cup B) - (A \cap B)\Bigr] \cup C$
						\begin{center}
							\begin{venndiagram3sets}[shade=circle area, tikzoptions={myvennoutline}, showframe=false]
								\fillANotB
								\fillBNotA
								\fillC
							\end{venndiagram3sets}
						\end{center}
				\end{enumerate}
			\end{examplebox}
			\subsection{Self-Assessment Exercises (Activity 4-4)}
				\begin{enumerate}
					\item
						\begin{enumerate}
							\item $(X \cup Y)'$
								\begin{center}
									$X \cup Y$\\
									\begin{venndiagram2sets}[shade=circle area, labelA=$X$, labelB=$Y$]
										\fillA
										\fillB
									\end{venndiagram2sets}\\
									$(X \cup Y)'$\\
									\begin{venndiagram2sets}[shade=circle area, labelA=$X$, labelB=$Y$]
										\fillNotAorB
									\end{venndiagram2sets}
								\end{center}
							\pagebreak
							\item $X' \cap Y'$
								\begin{center}
									$X'$\\
									\begin{venndiagram2sets}[shade=circle area, labelA=$X$, labelB=$Y$]
										\fillNotA
									\end{venndiagram2sets}\\
									$Y'$\\
									\begin{venndiagram2sets}[shade=circle area, labelA=$X$, labelB=$Y$]
										\fillNotB
									\end{venndiagram2sets}\\
									$X' \cap Y'$\\
									\begin{venndiagram2sets}[shade=circle area, labelA=$X$, labelB=$Y$]
										\fillNotAorB
									\end{venndiagram2sets}
								\end{center}
							\item $(X \cap Y)'$
								\begin{center}
									$X \cap Y$\\
									\begin{venndiagram2sets}[shade=circle area, labelA=$X$, labelB=$Y$]
										\fillACapB
									\end{venndiagram2sets}\\
									$(X \cap Y)'$\\
									\begin{venndiagram2sets}[shade=circle area, labelA=$X$, labelB=$Y$]
										\fillNotAorNotB
									\end{venndiagram2sets}
								\end{center}
							\pagebreak
							\item $X' \cap Y'$
								\begin{center}
									$X'$\\
									\begin{venndiagram2sets}[shade=circle area, labelA=$X$, labelB=$Y$]
										\fillNotA
									\end{venndiagram2sets}\\
									$Y'$\\
									\begin{venndiagram2sets}[shade=circle area, labelA=$X$, labelB=$Y$]
										\fillNotB
									\end{venndiagram2sets}\\
									$X' \cup Y'$\\
									\begin{venndiagram2sets}[shade=circle area, labelA=$X$, labelB=$Y$]
										\fillNotA
										\fillNotB
									\end{venndiagram2sets}
								\end{center}
						\end{enumerate}
					\pagebreak
					\item
						\begin{enumerate}
							\item $X - (Y \cup Z)$
								\begin{center}
									$X$\\
									\begin{venndiagram3sets}[shade=circle area, labelA=$X$, labelB=$Y$, labelC=$Z$]
										\fillA
									\end{venndiagram3sets}\\
									$Y \cup Z$\\
									\begin{venndiagram3sets}[shade=circle area, labelA=$X$, labelB=$Y$, labelC=$Z$]
										\fillB
										\fillC
									\end{venndiagram3sets}\\
									$X - (Y \cup Z)$\\
									\begin{venndiagram3sets}[shade=circle area, labelA=$X$, labelB=$Y$, labelC=$Z$]
										\fillOnlyA
									\end{venndiagram3sets}\\
								\end{center}
							\pagebreak
							\item $(X - Y) \cup (X - Z)$
								\begin{center}
									$(X - Y)$\\
									\begin{venndiagram3sets}[shade=circle area, labelA=$X$, labelB=$Y$, labelC=$Z$]
										\fillANotB
									\end{venndiagram3sets}\\
									$(X - Z)$\\
									\begin{venndiagram3sets}[shade=circle area, labelA=$X$, labelB=$Y$, labelC=$Z$]
										\fillANotC
									\end{venndiagram3sets}\\
									$(X - Y) \cup (X - Z)$\\
									\begin{venndiagram3sets}[shade=circle area, labelA=$X$, labelB=$Y$, labelC=$Z$]
										\fillANotB
										\fillANotC
									\end{venndiagram3sets}\\
								\end{center}
							\pagebreak
							\item $X \cap (Y - Z)$
								\begin{center}
									$X$\\
									\begin{venndiagram3sets}[shade=circle area, labelA=$X$, labelB=$Y$, labelC=$Z$]
										\fillA
									\end{venndiagram3sets}\\
									$Y - Z$\\
									\begin{venndiagram3sets}[shade=circle area, labelA=$X$, labelB=$Y$, labelC=$Z$]
										\fillBNotC
									\end{venndiagram3sets}\\
									$X \cap (Y - Z)$\\
									\begin{venndiagram3sets}[shade=circle area, labelA=$X$, labelB=$Y$, labelC=$Z$]
										\fillACapBNotC
									\end{venndiagram3sets}\\
								\end{center}
							\pagebreak
							\item $(X \cap Y) - (X \cap Z)$
								\begin{center}
									$X \cap Y$\\
									\begin{venndiagram3sets}[shade=circle area, labelA=$X$, labelB=$Y$, labelC=$Z$]
										\fillACapB
									\end{venndiagram3sets}\\
									$X \cap Z$\\
									\begin{venndiagram3sets}[shade=circle area, labelA=$X$, labelB=$Y$, labelC=$Z$]
										\fillACapC
									\end{venndiagram3sets}\\
									$(X \cap Y) - (X \cap Z)$\\
									\begin{venndiagram3sets}[shade=circle area, labelA=$X$, labelB=$Y$, labelC=$Z$]
										\fillACapBNotC
									\end{venndiagram3sets}\\
								\end{center}
							\pagebreak
							\item $X \cap (Y + Z)$
								\begin{center}
									$X$\\
									\begin{venndiagram3sets}[shade=circle area, labelA=$X$, labelB=$Y$, labelC=$Z$]
										\fillA
									\end{venndiagram3sets}\\
									$Y + Z$\\
									\begin{venndiagram3sets}[shade=circle area, labelA=$X$, labelB=$Y$, labelC=$Z$]
										\fillBNotC
										\fillCNotB
									\end{venndiagram3sets}\\
									$X \cap (Y + Z)$\\
									\begin{venndiagram3sets}[shade=circle area, labelA=$X$, labelB=$Y$, labelC=$Z$]
										\fillACapBNotC
										\fillACapCNotB
									\end{venndiagram3sets}\\
								\end{center}
							\pagebreak
							\item $(X \cap Y) + (X \cap Z)$
								\begin{center}
									$X \cap Y$\\
									\begin{venndiagram3sets}[shade=circle area, labelA=$X$, labelB=$Y$, labelC=$Z$]
										\fillACapB
									\end{venndiagram3sets}\\
									$X \cap Z$\\
									\begin{venndiagram3sets}[shade=circle area, labelA=$X$, labelB=$Y$, labelC=$Z$]
										\fillACapC
									\end{venndiagram3sets}\\
									$(X \cap Y) + (X \cap Z)$\\
									\begin{venndiagram3sets}[shade=circle area, labelA=$X$, labelB=$Y$, labelC=$Z$]
										\fillACapBNotC
										\fillACapCNotB
									\end{venndiagram3sets}\\
								\end{center}
						\end{enumerate}
				\end{enumerate}
		\pagebreak
		\section{Proofs}
			For proofs with sets, one needs to prove that the sets have exactly the same elements. For this, one needs to show that each half of the equation is equal to the other half: one needs to show both forwards and backwards. However, this can be abbreviated using iff.
			\begin{examplebox}
				(Long Way:) Prove that for all subsets $A$ and $B$ of $U$, $A \cup B = B \cup A$
				\begin{proof}
					Show $(A \cup B) \subseteq (B \cup A)$
					\begin{tabbing}
						Let $\qquad$ \=$x \in (A \cup B)$\\
						If \>$x \in (A \cup B)$\\
						then \> $x \in A$ or $x \in B$\\
						i.e. \> $x \in B$ or $x \in A$\\
						i.e. \> $x \in (B \cup A)$
					\end{tabbing}
					$\therefore$ if $x \in (A \cup B)$, then $x \in (B \cup A)$,\\
					$\therefore (A \cup B) \subseteq (B \cup A)$.

					\vspace{7mm}
					Show $(B \cup A) \subseteq (A \cup B)$
					\begin{tabbing}
						Let $\qquad$ \=$x \in (B \cup A)$\\
						If \>$x \in (B \cup A)$\\
						then \> $x \in B$ or $x \in A$\\
						i.e. \> $x \in A$ or $x \in B$\\
						i.e. \> $x \in (A \cup B)$
					\end{tabbing}
					$\therefore$ if $x \in (B \cup A)$, then $x \in (A \cup B)$,\\
					$\therefore (B \cup A) \subseteq (A \cup B)$.
					
					\vspace{5mm}
					$\therefore A \cup B = B \cup A$
				\end{proof}
			\end{examplebox}
			Using iff can shorten this, but be careful!
			\begin{examplebox}
				\begin{tabbing}
					$\quad$ \=$x \in (X \cup Y)'$\\
					iff \>$x \notin (X \cup Y)$\\
					iff \>$x \notin X$ and $x \notin Y$\\
					iff \>$x \in X'$ and $x \in Y'$\\
					iff \>$x \in X' \cap Y'$
				\end{tabbing}
				\begin{tabbing}
					$\quad$ \=$x \in (X \cap Y)'$\\
					iff \> $x \notin (X \cap Y)$\\
					iff \> $x \notin X$ or $x \notin Y$\\
					iff \> $x \in X'$ or $x \in Y'$\\
					iff \> $x \in X' \cup Y'$
				\end{tabbing}
			\end{examplebox}
			\pagebreak
			\subsection{Self-Assessment Exercises (4-6)}
				\begin{enumerate}[label=(\alph*)]
					\item $(X')' = X$\\
						Let $x \in (X')'$.
						\begin{tabbing}
							$\quad$ \= $x \in (X')'$\\
							iff \> $x \notin X'$\\
							iff \> $x \in X$\\
							$\therefore$ \> $(X')' = X$
						\end{tabbing}
					\item $X - (Y \cap W) = (X - Y) \cup (X - W)$\\
						Let $x \in X - (Y \cap W)$.
						\begin{tabbing}
							$\quad$ \= $x \in X - (Y \cap W)$\\
							iff \> $x \in X$ and $x \notin (Y \cap W)$\\
							iff \> $x \in X$ and $x \in Y'$ or $x \in W'$\\
							iff \> $\Bigl(x \in X$ and $x \in Y'\Bigr)$ or $\Bigl(x \in X$ and $x \in W'\Bigr)$\\
							iff \> $\Bigl(x \in (X - Y)\Bigr)$ or $\Bigl(x \in (X - W)\Bigr)$\\
							iff \> $x \in (X - Y) \cup (X - W)$\\
							$\therefore$ \> $X - (Y \cap W) = (X - Y) \cup (X - W)$
						\end{tabbing}
					\item $X \cap (Y \cap W) = (X \cap Y) \cap W$\\
						Let $x \in X \cap (Y \cap W)$.
						\begin{tabbing}
							$\quad$ \= $x \in X \cap (Y \cap W)$\\
							iff \> $x \in X$ and $x \in (Y \cap W)$\\
							iff \> $x \in X$ and $x \in Y$ and $x \in W$\\
							iff \> $(x \in X$ and $x \in Y)$ and $x \in W$\\
							iff \> $x \in (X \cap Y)$ and $x \in W$\\
							iff \> $x \in (X \cap Y) \cap W$\\
							$\therefore$ \> $X \cap (Y \cap W) = (X \cap Y) \cap W$
						\end{tabbing}
					\item $X \cap (Y \cup W) = (X \cap Y) \cup (X \cap W)$\\
						Let $x \in X \cap (Y \cup W)$
						\begin{tabbing}
							$\quad$ \= $x \in X \cap (Y \cup W)$\\
							iff \> $x \in X$ and $x \in (Y \cup W)$\\
							iff \> $x \in X$ and ($x \in Y$ or $x \in W$)\\
							iff \> ($x \in X$ and $x \in Y$) or ($x \in X$ and $x \in W$)\\
							iff \> ($x \in (X \cap Y)$) or ($x \in (X \cap W)$)\\
							iff \> $x \in (X \cap Y) \cup (X \cap W)$\\
							$\therefore$ \> $X \cap (Y \cup W) = (X \cap Y) \cup (X \cap W)$
						\end{tabbing}
				\end{enumerate}
			\pagebreak
			\subsection{Proofs Continued}
			In order to prove that two sets are not equal, one needs to just provide a \textbf{counterexample} - an element that is in one set that is not in the other.
	\end{document}